ratchet/Denote/Rules.lean
@@ -21,6 +21,7 @@ import Denote.Rules.CaseEq
 import Denote.Rules.ClsToS
 import Denote.Rules.ClassOf
 import Denote.Rules.NewInst
+import Denote.Rules.Raise
 import Denote.Sem.Frame
 
 /-!
